* Chapter 1
** Propositional Logic
*** Converse Contrapositive and Inverse (p -> q)
**** Coverse
***** q \rightarrow  p
**** Contrapositive
***** q \rightarrow \textlnot{}p
**** Inverse
***** \textlnot{}p \rightarrow \textlnot{}q
** Applications of Propositional Logic
*** Examples of turning sentences into propositional Logic.
** Propositional Equivalences
*** Logical Equivalences
|---------------------------+---------------------------------+----------------------|
| p\wedge T                 | p                               | Identity Laws        |
| p\vee F                   | p                               |                      |
|---------------------------+---------------------------------+----------------------|
| p\vee T                   | T                               | Domination Laws      |
| p\wedge F                 | F                               |                      |
|---------------------------+---------------------------------+----------------------|
| p\vee p                   | p                               | Idempotent Laws      |
| p\wedge p                 | p                               |                      |
|---------------------------+---------------------------------+----------------------|
| \textlnot{}(\textlnot{}p) | p                               | Double Negation Laws |
|---------------------------+---------------------------------+----------------------|
| p\vee q                   | q\vee p                         | Commutative Laws     |
| p\wedge q                 | q \wedge p                      |                      |
|---------------------------+---------------------------------+----------------------|
| (p\vee q)\vee r           | p\vee (q\vee r)                 | Associative Laws     |
| (p\wedge q) \wedge r      | p \wedge (q \wedge r)           |                      |
|---------------------------+---------------------------------+----------------------|
| p\vee (q\wedge r)         | (p\vee q) \wedge (p\vee r)      | Distributive Laws    |
| p \wedge (q\vee r)        | (p\wedge q)\vee (p \wedge r)    |                      |
|---------------------------+---------------------------------+----------------------|
| \textlnot{}(p\wedge q)    | \textlnot{}p\vee \textlnot{}q   | De Morgans Laws      |
| \textlnot{}(p v q)        | \textlnot{}p\wedge \textlnot{}q |                      |
|---------------------------+---------------------------------+----------------------|
| p\vee (p\wedge q)         | p                               | Absorption Laws      |
| p \wedge (p\vee q)        | p                               |                      |
|---------------------------+---------------------------------+----------------------|
| p v \textlnot{}p          | T                               | Negation Laws        |
| p\wedge \textlnot{}p      | F                               |                      |
|---------------------------+---------------------------------+----------------------|

*** Logical Equivelances Involving Conditional Statements
|-------------------------------------------+-----------------------------------------|
| p \rightarrow q                           | \textlnot{}p\vee q                      |
|-------------------------------------------+-----------------------------------------|
| p \rightarrow q                           | \textlnot{}q \rightarrow \textlnot{}p   |
|-------------------------------------------+-----------------------------------------|
| p\vee q                                   | \textlnot{}p \rightarrow q              |
|-------------------------------------------+-----------------------------------------|
| p\wedge  q                                | \textlnot{}(p \rightarrow \textlnot{}q) |
|-------------------------------------------+-----------------------------------------|
| \textlnot{}(p \rightarrow q)              | p\wedge q                               |
|-------------------------------------------+-----------------------------------------|
| (p \rightarrow q)\wedge (p \rightarrow r) | p \rightarrow (q \wedge r)              |
|-------------------------------------------+-----------------------------------------|
| (p \rightarrow r)\wedge (q \rightarrow r) | (p\vee q) \rightarrow r                 |
|-------------------------------------------+-----------------------------------------|
| (p \rightarrow q)\vee (p \rightarrow r)   | p \rightarrow (q\vee r)                 |
|-------------------------------------------+-----------------------------------------|
| (p \rightarrow r)\vee (q \rightarrow r)   | (p\wedge q) \rightarrow r               |
|-------------------------------------------+-----------------------------------------|

*** Logical Equivalences Involving Biconditional Statements
|----------------------------------+----------------------------------------------------|
| p \leftrightarrow q              | (p \rightarrow q)\wedge (q \rightarrow p)          |
|----------------------------------+----------------------------------------------------|
| p \leftrightarrow q              | \textlnot{}p \leftrightarrow \textlnot{}q          |
|----------------------------------+----------------------------------------------------|
| p \leftrightarrow q              | (p\wedge q)\vee (\textlnot{}p \wedge \textlnot{}q) |
|----------------------------------+----------------------------------------------------|
| \textlnot{}(p \leftrightarrow q) | p \leftrightarrow \textlnot{}q                     |
|----------------------------------+----------------------------------------------------|

** Predicates and Quantifiers
*** Quantifiers
**** Universal Quantifer 
***** \forall(x) P(x) 
****** Definition: For all x in the universe P(x) is true;
****** Negation
******* \textlnot{}\forall(x) P(x) can also be written as \exists\textlnot{} P(x)
******* There exists an x such that P(x) is false
**** Existential Quantifer
***** \exists(x) P(x)
****** Definition: For all x in the universe P(x) is true for at least one x;
****** Negation
******* \textlnot{}\exists(x) P(x) can also be written as \forall\textlnot{} P(x)
******* All x in the universe make P(x) false
** Nested Quantifers
*** Nested Quantifiers can be used when there are multiple variables such as x and y
**** \forall (x) \exists (y) (x + y = 0)
*** Quantification of Two Variables
|--------------------------------+--------------------------------+----------------------------------|
| Statement                      | When True                      | When False                       |
|--------------------------------+--------------------------------+----------------------------------|
| \forall (x) \forall (y) P(x,y) | P(x,y) is true for every pair  | When there is a x,y              |
|                                |                                | for which P(x,y) is false        |
|--------------------------------+--------------------------------+----------------------------------|
| \forall (x) \exists (y) P(x,y) | For every x there is a y       | When there is an x such          |
|                                | for which P(x,y) is true       | that P(x,y) is false for every y |
|--------------------------------+--------------------------------+----------------------------------|
| \exists (x) \forall (y) P(x,y) | There is an x for which P(x,y) | When for every x there is a y    |
|                                | is true for every y            | for which P(x,y) is false        |
|--------------------------------+--------------------------------+----------------------------------|
| \exists (x) \exists (y) P(x,y) | There is a pair for x,y        | P(x,y) is false for              |
| \exists (y) \exists (x) P(x,y) | for which P(x,y) is true       | every pair of x and y            |
|--------------------------------+--------------------------------+----------------------------------|

** Rules of Inference 
*** 
** Introduction to Proofs
** Proof methods and Strategy
* Chapter 2
** Sets
** Set Operations
** Functions
** Sequences and Summations
** Cardinality of Sets
** Matrices



\emptyset
